withPureSteps/NonSpec.v
@@ -7,30 +7,66 @@ Definition pHeap := heap pivar_state.
 
 Inductive pctxt : Type :=
 |pbindCtxt : pctxt -> ptrm -> pctxt
-|phandleCtxt : pctxt -> ptrm -> pctxt 
-|pholeCtxt : pctxt.
+|phandleCtxt : pctxt -> ptrm -> pctxt
+|pappCtxt : pctxt -> ptrm -> pctxt 
+|pappValCtxt : pctxt -> ptrm -> pctxt 
+|ppairCtxt : pctxt -> ptrm -> pctxt 
+|ppairValCtxt : pctxt -> ptrm -> pctxt
+|pfstCtxt : pctxt -> pctxt 
+|psndCtxt : pctxt -> pctxt  
+|pholeCtxt : pctxt
+.
 
-Fixpoint pdecompose (t:ptrm) : (pctxt * ptrm) :=
-  match t with
-      |pbind M N => let (E, M') := pdecompose M
-                    in (pbindCtxt E N, M')
-      |phandle M N => let (E, M') := pdecompose M
-                      in (phandleCtxt E N, M')
-      |_ => (pholeCtxt, t)
-  end. 
+Inductive pdecompose : ptrm -> pctxt -> ptrm -> Prop :=
+|pdecompBind : forall M N E M', pdecompose M E M' -> pdecompose (pbind M N) (pbindCtxt E N) M'
+|pdecompHandle : forall M M' N E, pdecompose M E M' -> pdecompose (phandle M N) (phandleCtxt E N) M'
+|pdecompApp : forall M N M' E, pval M = false -> pdecompose M E M' -> 
+                              pdecompose (papp M N) (pappCtxt E N) M'
+|pdecompAppVal : forall M N N' E, pval M = true -> pdecompose N E N' ->
+                                 pdecompose (papp M N) (pappValCtxt E M) N'
+|pdecompPair : forall M M' E N, pval M = false -> pdecompose M E M' ->
+                               pdecompose (ppair M N) (ppairCtxt E N) M'
+|pdecompValPair : forall M N N' E, pval M = true -> pval N = false -> pdecompose N E N' ->
+                                  pdecompose (ppair M N) (ppairValCtxt E M) N'
+|pdecompFst : forall M M' E, pdecompose M E M' -> pdecompose(pfst M) (pfstCtxt E) M'
+|pdecompSnd : forall M M' E, pdecompose M E M' -> pdecompose(psnd M) (psndCtxt E) M'
+|pdecompVal : forall M, pval M = true -> pdecompose M pholeCtxt M
+. 
 
 Fixpoint pfill (c:pctxt) (t:ptrm) : ptrm :=
   match c with
       |pbindCtxt E N => pbind (pfill E t) N
       |phandleCtxt E N => phandle (pfill E t) N
+      |pappCtxt E N => papp (pfill E t) N
+      |pappValCtxt E M => papp M (pfill E t)
+      |ppairCtxt E N => ppair (pfill E t) N
+      |ppairValCtxt E M => ppair M (pfill E t)
+      |pfstCtxt E => pfst (pfill E t)
+      |psndCtxt E => psnd (pfill E t)
       |pholeCtxt => t
   end. 
 
-Theorem pdecomposeEq : forall M E e, pdecompose M = (E, e) -> M = pfill E e. 
+Ltac helperTac :=
+  match goal with
+    |H:?x=?y |- _ => inversion H; subst; clear H
+    |H:forall M e, (?x,?y) = (M, e) -> ?z |- _ => assert(EQ:(x,y)=(x,y)) by auto; apply H in EQ
+  end. 
+
+Theorem pdecomposeEq : forall M E e, pdecompose M E e -> M = pfill E e. 
 Proof.
-  induction M; intros; simpl in *; inversion H; try reflexivity; try solve[
-  destruct (pdecompose M1); inversion H; inversion H1; subst;  
-   assert((p,e)=(p,e)) by reflexivity; apply IHM1 in H0; subst; reflexivity]. 
+  induction M; intros; try solve[inversion H; subst; auto].  
+  {inversion H; subst; auto. simpl. apply IHM1 in H5. subst; auto. 
+   apply IHM2 in H6; subst; auto. }
+  {inversion H; subst; auto. apply IHM1 in H5; subst; auto. apply IHM2 in H5; subst; auto. }
+  {inversion H; subst; auto. apply IHM1 in H4; subst; auto. }
+  {inversion H; subst; auto. apply IHM1 in H4; subst; auto. }
+  {inversion H; subst; auto. apply IHM in H1; subst; auto. }
+  {inversion H; subst; auto. apply IHM in H1; subst; auto. }
+Qed. 
+
+Theorem pdecomposedVal : forall t E e, pdecompose t E e -> pval e = true. 
+Proof.
+  induction t; intros; try solve[inversion H; subst; auto]; try solve[inversion H; subst; eauto]. 
 Qed. 
 
 Definition pPool := Ensemble ptrm. 
@@ -42,33 +78,42 @@ Inductive pconfig : Type :=
 |pOK : pHeap -> pPool -> pPool -> pconfig. 
 
 Inductive pstep : pHeap -> pPool -> pPool -> pconfig -> Prop :=
+|PBetaRed : forall t E e arg h T,
+              pdecompose t (pappValCtxt E (plambda e)) arg -> pval arg = true ->
+              pstep h T (pSingleton t) (pOK h T (pSingleton (pfill E (popen 0 arg e))))
+|pProjectL : forall V1 V2 h T t E,
+               pdecompose t (pfstCtxt E) (ppair V1 V2) -> pval V1 = true -> pval V2 = true ->
+               pstep h T (pSingleton t) (pOK h T (pSingleton (pfill E V1)))
+|pProjectR : forall V1 V2 h T t E,
+               pdecompose t (psndCtxt E) (ppair V1 V2) -> pval V1 = true -> pval V2 = true ->
+               pstep h T (pSingleton t) (pOK h T (pSingleton (pfill E V2)))
 |PBind : forall E t M N h T, 
-            pdecompose t = (pbindCtxt E N, pret M) -> 
+            pdecompose t (pbindCtxt E N) (pret M) -> 
            pstep h T (pSingleton t) (pOK h T (pSingleton(pfill E(papp N M))))
 |PBindRaise : forall E t M N h T,
-                 pdecompose t = (pbindCtxt E N, praise M) -> 
+                 pdecompose t (pbindCtxt E N) (praise M) -> 
                 pstep h T (pSingleton t) (pOK h T (pSingleton (pfill E(praise M))))
 |pHandle : forall E t M N h T,
-              pdecompose t = (phandleCtxt E N, praise M) -> 
+              pdecompose t (phandleCtxt E N) (praise M) -> 
              pstep h T (pSingleton t) (pOK h T (pSingleton (pfill E(papp N M))))
 |pHandleRet : forall E t M N h T,
-                 pdecompose t = (phandleCtxt E N, pret M) -> 
+                 pdecompose t (phandleCtxt E N) (pret M) -> 
                 pstep h T (pSingleton t) (pOK h T (pSingleton (pfill E(pret M))))
 |pFork : forall E t M h T,
-            pdecompose t = (E, pfork M) -> 
+            pdecompose t E (pfork M) -> 
            pstep h T (pSingleton t) (pOK h T (Couple ptrm (pfill E(pret punit)) M))
 |PGet : forall E M t h T x,
-           heap_lookup x h = Some(pfull M) -> pdecompose t = (E, pget (pfvar x)) -> 
+           heap_lookup x h = Some(pfull M) -> pdecompose t E (pget (pfvar x)) -> 
           pstep h T (pSingleton t) (pOK h T (pSingleton (pfill E(pret M))))
 |PPut : forall E t M h h' T x,
-           pdecompose t = (E, pput (pfvar x) M) -> heap_lookup x h = Some pempty ->
+           pdecompose t E (pput (pfvar x) M) -> heap_lookup x h = Some pempty ->
           h' = replace x (pfull M) h ->
           pstep h T (pSingleton t) (pOK (replace x (pfull M) h) T (pSingleton (pfill E (pret punit))))
 |PPutError : forall E t M h T x N,
-               pdecompose t = (E, pput (pfvar x) M) -> heap_lookup x h = Some (pfull N) ->
+               pdecompose t E (pput (pfvar x) M) -> heap_lookup x h = Some (pfull N) ->
                pstep h T (pSingleton t) pError
 |PNew : forall E t h h' T x,
-             pdecompose t = (E, pnew) -> (x, h') = extend pempty h ->
+             pdecompose t E pnew -> (x, h') = extend pempty h ->
              pstep h T (pSingleton t) (pOK h' T (pSingleton (pfill E (pret (pfvar x)))))
 |PTerminate : forall h T M, pstep h T (pSingleton (pret M)) (pOK h T (Empty_set ptrm))
                 
@@ -97,10 +142,34 @@ Proof.
   assumption. Qed.   
 
 
+(*Evaluation Context well formedness with respect to a particular term*)
+Inductive pctxtWF : ptrm -> pctxt -> Prop :=
+|pbindWF : forall e E N, pctxtWF e E -> pctxtWF e (pbindCtxt E N)
+|phandleCtxtWF : forall e E N, pctxtWF e E -> pctxtWF e (phandleCtxt E N)
+|pappCtxtWF : forall e E N, pctxtWF e E -> pval (pfill E e) = false -> pctxtWF e (pappCtxt E N)
+|pappValCtxtWF : forall e E N, pctxtWF e E -> pval N = true -> pctxtWF e (pappValCtxt E N)
+|ppairCtxtWF : forall e E N, pctxtWF e E -> pval (pfill E e) = false -> pctxtWF e (ppairCtxt E N)
+|ppairValCtxtWF : forall e E N, pctxtWF e E -> pval N = true -> pval (pfill E e) = false -> 
+                               pctxtWF e (ppairValCtxt E N)
+|psndCtxtWF : forall e E, pctxtWF e E -> pctxtWF e (psndCtxt E)
+|pfstCtxtWF : forall e E, pctxtWF e E -> pctxtWF e (pfstCtxt E)
+|pholeCtxtWF : forall e, pval e = true -> pctxtWF e pholeCtxt
+.
 
+Theorem pdecomposeDecomposed : forall E e, pctxtWF e E ->
+                                           pdecompose e pholeCtxt e -> 
+                                           pdecompose (pfill E e) E e.
+Proof.
+  induction E; intros; auto; try solve[inversion H; subst; simpl; constructor; apply IHE; auto]; 
+  try solve[inversion H; subst; simpl; constructor; auto].  
+Qed.
 
+Hint Constructors pctxtWF. 
 
-
-
-
-
+Theorem pdecomposeWF : forall t E e, pdecompose t E e -> pctxtWF e E. 
+Proof.
+  intros. induction H; auto. 
+  {constructor. assumption. apply pdecomposeEq in H0. rewrite <- H0. auto. }
+  {constructor. assumption. apply pdecomposeEq in H0. rewrite <- H0. auto. }
+  {constructor. assumption. assumption. apply pdecomposeEq in H1. rewrite <- H1. auto. }
+Qed. 
