withPureSteps/nonspeculativeImpliesSpeculative.v
@@ -50,13 +50,6 @@ Ltac invertHyp :=
        eapply ctxtErasureDeterminism in H; try eassumption; subst; try invertHyp
   end. 
 
-Theorem pdecomposeDecomposed : forall E e, pdecompose e = (pholeCtxt, e) -> 
-                                           pdecompose (pfill E e) = (E, e).
-Proof.
-  induction E; intros; auto;
-  simpl; apply IHE in H; destruct (pdecompose(pfill E e)); inversion H; auto. 
-Qed. 
-
 Ltac instantiateHeap :=
   match goal with
       |H:pstep ?H ?T ?t (pOK ?H ?T' ?t') |- _ => assert(EH:exists H', eraseHeap H' H) by apply eHeap; 
@@ -64,22 +57,7 @@ Ltac instantiateHeap :=
                                           exists newHeap
       |H:pstep ?H ?T ?t (pOK ?H' ?T' ?t') |- _ => assert(EH:exists H', eraseHeap H' H) by apply eHeap;
                                           inversion EH as[newHeap heapHyp]; exists newHeap
-  end. 
-
-Ltac instantiateContext := 
-  match goal with 
-      |H:pdecompose ?t = (pbindCtxt ?E ?N, ?e) |- _ => 
-       assert(CTXT:exists E', eraseContext E' tEmptySet E) by apply eCtxt; inversion CTXT; clear CTXT;
-       assert(NHyp:exists N', eraseTerm N' tEmptySet N) by apply eTerm; inversion NHyp; clear NHyp;
-       assert(eHyp:exists e', eraseTerm e' tEmptySet e) by apply eTerm; inversion eHyp; clear eHyp
-      |H:pdecompose ?t = (phandleCtxt ?E ?N, ?e) |- _ => 
-       assert(CTXT:exists E', eraseContext E' tEmptySet E) by apply eCtxt; inversion CTXT; clear CTXT;
-       assert(NHyp:exists N', eraseTerm N' tEmptySet N) by apply eTerm; inversion NHyp; clear NHyp;
-       assert(eHyp:exists e', eraseTerm e' tEmptySet e) by apply eTerm; inversion eHyp; clear eHyp
-      |H:pdecompose ?t = (?E, ?e) |- _ =>
-       assert(CTXT:exists E', eraseContext E' tEmptySet E) by apply eCtxt; inversion CTXT; clear CTXT;
-       assert(eHyp:exists e', eraseTerm e' tEmptySet e) by apply eTerm; inversion eHyp; clear eHyp
-  end.
+  end.  
 
 Ltac instantiatePool :=
   match goal with
@@ -104,8 +82,6 @@ Proof.
    subst. constructor. assumption. assumption. constructor. eapply IHU. assumption. assumption. }
   {simpl in *. inversion H. }
 Qed. 
-
-
 
 Ltac proveDisjoint :=
   unfold tSingleton in *;
@@ -225,106 +201,301 @@ Proof.
   {simpl in *. inversion H1; inversion H2; cleanup. repeat constructor. }
 Qed. 
 
+Theorem eraseFill' : forall E e E' e' T, eraseTerm e T e' -> eraseContext E T E' ->
+                                       eraseTerm (fill E e) T (pfill E' e').
+Proof.
+  intros. generalize dependent e. generalize dependent e'. induction H0; intros; try solve[simpl; auto]. 
+  {simpl. econstructor. apply IHeraseContext. assumption. reflexivity. eassumption. 
+   eassumption. }
+Qed. 
+
+Inductive uneraseTerm : ptrm -> trm -> Prop :=
+|uneraseFVar : forall i, uneraseTerm (pfvar i) (fvar i)
+|uneraseBVar : forall i, uneraseTerm (pbvar i) (bvar i)
+|uneraseUnit : uneraseTerm punit unit
+|unerasePair : forall e1 e1' e2 e2', uneraseTerm e1' e1 -> uneraseTerm e2' e2 ->
+                                     uneraseTerm (ppair e1' e2') (pair_ e1 e2)
+|uneraseLambda : forall e e', uneraseTerm e' e -> uneraseTerm (plambda e') (lambda e)
+|uneraseApp : forall e1 e1' e2 e2', uneraseTerm e1' e1 -> uneraseTerm e2' e2 ->
+                                    uneraseTerm (papp e1' e2') (app e1 e2)
+|uneraseRet : forall e e', uneraseTerm e' e -> uneraseTerm (pret e') (ret e)
+|uneraseBind : forall e1 e1' e2 e2', uneraseTerm e1' e1 -> uneraseTerm e2' e2 ->
+                                     uneraseTerm (pbind e1' e2') (bind e1 e2)
+|uneraseFork : forall e e', uneraseTerm e' e -> uneraseTerm (pfork e') (fork e)
+|uneraseNew : uneraseTerm pnew new
+|unerasePut : forall e1 e1' e2 e2', uneraseTerm e1' e1 -> uneraseTerm e2' e2 ->
+                                    uneraseTerm (pput e1' e2') (put e1 e2)
+|uneraseGet : forall e e', uneraseTerm e' e -> uneraseTerm (pget e') (get e)
+|uneraseRaise : forall e e', uneraseTerm e' e -> uneraseTerm (praise e') (raise e)
+|uneraseHandle : forall e1 e1' e2 e2', uneraseTerm e1' e1 -> uneraseTerm e2' e2 ->
+                                       uneraseTerm (phandle e1' e2') (handle e1 e2)
+|uneraseDone : forall e e', uneraseTerm e' e -> uneraseTerm (pdone e') (done e)
+|uneraseFst : forall e e', uneraseTerm e' e -> uneraseTerm (pfst e') (fst e)
+|uneraseSnd : forall e e', uneraseTerm e' e -> uneraseTerm (psnd e') (snd e)
+.
+
+Inductive uneraseCtxt : pctxt -> ctxt -> Prop :=
+|uneraseBindCtxt : forall E E' N N', uneraseTerm N' N -> uneraseCtxt E' E -> 
+                                     uneraseCtxt (pbindCtxt E' N') (bindCtxt E N)
+|uneraseHandleCtxt : forall E E' N N', uneraseTerm N' N -> uneraseCtxt E' E -> 
+                                       uneraseCtxt (phandleCtxt E' N') (handleCtxt E N)
+|uneraseAppCtxt : forall E E' N N', uneraseTerm N' N -> uneraseCtxt E' E -> 
+                                       uneraseCtxt (pappCtxt E' N') (appCtxt E N)
+|uneraseAppValCtxt : forall E E' N N', uneraseTerm N' N -> uneraseCtxt E' E -> 
+                                       uneraseCtxt (pappValCtxt E' N') (appValCtxt E N)
+|unerasePairCtxt : forall E E' N N', uneraseTerm N' N -> uneraseCtxt E' E -> 
+                                       uneraseCtxt (ppairCtxt E' N') (pairCtxt E N)
+|unerasePairValCtxt : forall E E' N N', uneraseTerm N' N -> uneraseCtxt E' E -> 
+                                       uneraseCtxt (ppairValCtxt E' N') (pairValCtxt E N)
+|uneraseFstCtxt : forall E E', uneraseCtxt E' E -> uneraseCtxt (pfstCtxt E') (fstCtxt E)
+|uneraseSndCtxt : forall E E', uneraseCtxt E' E -> uneraseCtxt (psndCtxt E') (sndCtxt E)
+|uneraseHoleCtxt : uneraseCtxt pholeCtxt holeCtxt
+.
+
+Hint Constructors uneraseTerm uneraseCtxt. 
+
+Theorem eUneraseTerm : forall e', exists e, uneraseTerm e' e.
+Proof.
+  induction e'; try solve[repeat econstructor]; try solve[invertExists; econstructor; eauto].  
+Qed. 
+
+Theorem eUneraseCtxt : forall E', exists E, uneraseCtxt E' E. 
+Proof.
+  induction E'; try solve[assert(exists p', uneraseTerm p p') by apply eUneraseTerm; invertExists; 
+  econstructor; eauto]; try solve[invertExists; econstructor; eauto]. 
+  econstructor. eauto. Qed. 
+
+Theorem eraseOpen : forall e1 e2 e1' e2' T n, eraseTerm e1 T e1' -> eraseTerm e2 T e2' ->
+                                              eraseTerm (open n e2 e1) T (popen n e2' e1'). 
+Proof.
+  induction e1; intros; try solve[inversion H; subst; auto];
+  try solve[inversion H; subst; simpl; constructor; apply IHe1; auto]; 
+  try solve[inversion H; subst; simpl; constructor; [apply IHe1_1; auto| apply IHe1_2; auto]].
+  {inversion H; subst. simpl. destruct (beq_nat n i); auto. }
+  {inversion H; subst. simpl. constructor. apply IHe1_2; auto. apply IHe1_1; auto. }
+  {inversion H; subst. simpl. replace  (popen (S n) e2' (incBV 1 e2'0)) with (incBV 1 (popen n e2' e2'0)). 
+   constructor. apply IHe1_1. assumption. assumption. admit. admit. }
+  {inversion H; subst. admit. }
+Qed. 
+
+Theorem pvalImpliesVal : forall e T e', eraseTerm e T e' -> pval e' = true -> val e = true. 
+Proof.
+  intros. induction H; auto. 
+  {simpl. apply andb_true_iff. simpl in H0. apply andb_true_iff in H0. inversion H0. 
+   split. apply IHeraseTerm1. auto. apply IHeraseTerm2; auto. }
+Qed. 
+
+Theorem decomposeVal : forall E e, ctxtWF e E -> val e = true -> decompose (fill E e) E e. 
+Proof.
+  intros. induction H; try solve[simpl; constructor; auto]. Qed. 
+
+Ltac instantiateContext := 
+  match goal with 
+      |H:pdecompose ?t (pappValCtxt ?E ?N) ?e |- _ => 
+       assert(CTXT:exists E', uneraseCtxt E E') by apply eUneraseCtxt; 
+       assert(NHyp:exists N', uneraseTerm N N') by apply eUneraseTerm; 
+       assert(eHyp:exists e', uneraseTerm e e') by apply eUneraseTerm; invertExists
+      |H:pdecompose ?t (pfstCtxt ?E) ?e |- _ => 
+       assert(CTXT:exists E', uneraseCtxt E E') by apply eUneraseCtxt; 
+       assert(eHyp:exists e', uneraseTerm e e') by apply eUneraseTerm; invertExists
+      |H:pdecompose ?t (psndCtxt ?E) ?e |- _ => 
+       assert(CTXT:exists E', uneraseCtxt E E') by apply eUneraseCtxt; 
+         assert(eHyp:exists e', uneraseTerm e e') by apply eUneraseTerm; invertExists
+      |H:pdecompose ?t (pbindCtxt ?E ?N) ?e |- _ => 
+       assert(CTXT:exists E', uneraseCtxt E E') by apply eUneraseCtxt;
+       assert(NHyp:exists N', uneraseTerm N N') by apply eUneraseTerm; 
+       assert(eHyp:exists e', uneraseTerm e e') by apply eUneraseTerm; invertExists
+    |H:pdecompose ?t (phandleCtxt ?E ?N) ?e |- _ => 
+       assert(CTXT:exists E', uneraseCtxt E E') by apply eUneraseCtxt;
+       assert(NHyp:exists N', uneraseTerm N N') by apply eUneraseTerm; 
+       assert(eHyp:exists e', uneraseTerm e e') by apply eUneraseTerm; invertExists
+      |H:pdecompose ?t ?E ?e |- _ =>
+       assert(CTXT:exists E', uneraseCtxt E E') by apply eUneraseCtxt;
+       assert(eHyp:exists e', uneraseTerm e e') by apply eUneraseTerm; invertExists
+  end.
+
+Theorem eraseUneraseTerm : forall e e', uneraseTerm e' e -> eraseTerm e tEmptySet e'. 
+Proof.
+  intros. induction H; auto. Qed.
+
+Hint Resolve eraseUneraseTerm.  
+
+Theorem eraseUneraseCtxt : forall E E', uneraseCtxt E' E -> eraseContext E tEmptySet E'. 
+Proof.
+  intros. induction H; auto. Qed. 
+
+Hint Resolve eraseUneraseCtxt. 
+
+Theorem uneraseValEq : forall M M', uneraseTerm M' M -> val M = pval M'. 
+Proof.
+  intros. induction H; auto. simpl. rewrite IHuneraseTerm1. rewrite IHuneraseTerm2. auto. Qed. 
+
+Theorem uneraseFill : forall E E' e e', uneraseCtxt E' E -> uneraseTerm e' e -> 
+                                        uneraseTerm (pfill E' e') (fill E e).
+Proof.
+  intros. generalize dependent e. generalize dependent e'. induction H; intros; auto; 
+  try solve[simpl; constructor; auto]. Qed. 
+
+Theorem uneraseDecompose : forall E E' e e' t, pdecompose t E' e' -> uneraseCtxt E' E ->
+                                               uneraseTerm e' e -> decompose (fill E e) E e.
+Proof.
+  intros. generalize dependent E. generalize dependent e. induction H; intros; 
+  try solve[inversion H0; subst; simpl; constructor; eapply IHpdecompose; auto]. 
+  {inversion H2; subst. simpl. constructor. apply pdecomposeEq in H0. subst. 
+   rewrite <- H. apply uneraseValEq. apply uneraseFill; auto. apply IHpdecompose; auto. }
+  {inversion H2; subst. simpl. constructor. rewrite <- H. apply uneraseValEq. auto. 
+   apply IHpdecompose; auto. }
+  {inversion H2; subst. simpl. constructor. apply pdecomposeEq in H0. subst. 
+   rewrite <- H. apply uneraseValEq. apply uneraseFill; auto. apply IHpdecompose; auto. }
+  {inversion H3; subst. simpl. constructor. rewrite <- H. apply uneraseValEq; auto. 
+   apply pdecomposeEq in H1. subst. rewrite <- H0. apply uneraseValEq; auto.
+   apply uneraseFill; auto. apply IHpdecompose; auto. }
+  {inversion H0; subst. simpl. constructor. rewrite <- H. apply uneraseValEq. assumption. }
+Qed. 
+   
+
+Theorem extendSpeculatedHeap : forall H H' x1 x2 x3 PH' v v', 
+                                 speculateHeap H' H -> (x1, PH') = extend v H'->
+                                 (x2, x3) = extend v' H -> x1 = x2. 
+Admitted. 
+
 Theorem nonspecImpliesSpec : forall PH PH' PT pt pt',
                                pstep PH PT pt (pOK PH' PT pt') ->
                                exists H H' t t' T,
                                  eraseHeap H PH /\ eraseHeap H' PH' /\ erasePool T PT /\
                                  erasePool t pt /\ erasePool t' pt' /\ multistep H T t (OK H' T t').
 Proof.
-  intros. inversion H. 
-  {cleanup. instantiateHeap. instantiateContext. inversion H2; subst. invertHyp. 
-   assert(tid:tid); repeat constructor. 
-   exists (tSingleton (tid, nil, nil, fill (bindCtxt x x0) (ret e))). 
-   exists (tSingleton (tid, nil, nil, fill x (AST.app x0 e))). instantiatePool. 
-   repeat(split; try assumption). eraseEq. constructor. eraseEq. apply termErasePoolErase. 
-   eapply eraseFill. eapply pdecomposeDecomposed; eauto. assumption. constructor; eauto. 
-   rewrite <- ERASEHYP. constructor. econstructor. rewrite <- union_empty at 1. rewrite Union_commutative. 
-   reflexivity. proveDisjoint. constructor. apply decomposeDecomposed. auto. unfold tUnion. 
-   rewrite Union_commutative. rewrite union_empty. constructor. }
-  {cleanup. instantiateHeap. instantiateContext. assert(tid:tid); repeat constructor. 
-   exists(tSingleton(tid,nil,nil,fill (bindCtxt x x0) x1)). 
-   exists(tSingleton(tid,nil,nil,fill x x1)). instantiatePool. repeat(split; try assumption). 
-   eraseEq. constructor. eraseEq. apply termErasePoolErase. eapply eraseFill; eauto. 
-   apply pdecomposeDecomposed; auto. rewrite <- ERASEHYP. constructor. inversion H2; subst.
+  intros. inversion H.  
+  {cleanup. instantiateHeap. instantiateContext. inversion H1; subst.  
+   exists(tSingleton(Tid(0,0)nil, nil, nil, fill (appValCtxt x1 (lambda e0)) x)). 
+   exists (tSingleton(Tid(0,0)nil,nil,nil, fill x1 (open 0 x e0))). instantiatePool.  
+   repeat split; auto. eraseEq. apply termErasePoolErase. copy H5. apply pdecomposeEq in H5. 
+   subst. apply eraseFill; auto. rewrite <- ERASEHYP. constructor. eraseEq. apply termErasePoolErase. 
+   apply eraseFill; auto. apply eraseOpen; auto. rewrite <- ERASEHYP. constructor. 
    econstructor. rewrite <- union_empty at 1. rewrite Union_commutative. reflexivity. proveDisjoint. 
-   eapply BindRaise. eapply decomposeDecomposed. auto. unfold tUnion. rewrite Union_commutative. 
+   constructor. eapply uneraseDecompose; eauto. eapply pvalImpliesVal; eauto.
+   unfold tUnion. rewrite Union_commutative. rewrite union_empty. auto. }
+  {cleanup. instantiateHeap. instantiateContext. inversion H0; subst.  
+   exists(tSingleton(Tid(0,0)nil, nil, nil, fill (fstCtxt x0) (pair_ e1 e2))). 
+   exists (tSingleton(Tid(0,0)nil,nil,nil, fill x0 e1)). instantiatePool.  
+   repeat split; auto. eraseEq. apply termErasePoolErase. copy H2. apply pdecomposeEq in H2. 
+   subst. apply eraseFill; auto. rewrite <- ERASEHYP. constructor. eraseEq. constructor. 
+   econstructor. rewrite <- union_empty at 1. rewrite Union_commutative. reflexivity. proveDisjoint. 
+   eapply ProjL. eapply uneraseDecompose; eauto. eapply pvalImpliesVal; eauto.
+   eapply pvalImpliesVal; eauto. 
+   unfold tUnion. rewrite Union_commutative. rewrite union_empty. auto. }
+  {cleanup. instantiateHeap. instantiateContext. inversion H0; subst.  
+   exists(tSingleton(Tid(0,0)nil, nil, nil, fill (sndCtxt x0) (pair_ e1 e2))). 
+   exists (tSingleton(Tid(0,0)nil,nil,nil, fill x0 e2)). instantiatePool.  
+   repeat split; auto. eraseEq. apply termErasePoolErase. copy H2. apply pdecomposeEq in H2. 
+   subst. apply eraseFill; auto. rewrite <- ERASEHYP. constructor. eraseEq. constructor. 
+   econstructor. rewrite <- union_empty at 1. rewrite Union_commutative. reflexivity. proveDisjoint. 
+   eapply ProjR. eapply uneraseDecompose; eauto. eapply pvalImpliesVal; eauto.
+   eapply pvalImpliesVal; eauto. 
+   unfold tUnion. rewrite Union_commutative. rewrite union_empty. auto. }
+  {cleanup. instantiateHeap. instantiateContext. inversion H0; subst. 
+   exists (tSingleton (Tid(0,0)nil, nil, nil, fill (bindCtxt x1 x0) (ret e))). 
+   exists (tSingleton (Tid(0,0)nil, nil, nil, fill x1 (AST.app x0 e))). instantiatePool. 
+   repeat(split; try assumption). eraseEq. apply termErasePoolErase. apply pdecomposeEq in H4. subst. 
+   apply eraseFill; eauto. rewrite <- ERASEHYP. constructor. eraseEq. constructor. econstructor.
+   rewrite <- union_empty at 1. rewrite Union_commutative. 
+   reflexivity. proveDisjoint. apply Bind. eapply uneraseDecompose; eauto. unfold tUnion. 
+   rewrite Union_commutative. rewrite union_empty. constructor. }
+  {cleanup. instantiateHeap. instantiateContext. inversion H0; subst. 
+   exists(tSingleton(Tid(0,0)nil,nil,nil,fill (bindCtxt x1 x0) (raise e))). 
+   exists(tSingleton(Tid(0,0)nil,nil,nil,fill x1 (raise e))). instantiatePool. repeat(split; try assumption). 
+   eraseEq. apply termErasePoolErase. apply pdecomposeEq in H4; subst. apply eraseFill; eauto. 
+   rewrite <- ERASEHYP. constructor. eraseEq. constructor. 
+   econstructor. rewrite <- union_empty at 1. rewrite Union_commutative. reflexivity. proveDisjoint. 
+   eapply BindRaise. eapply uneraseDecompose; eauto. unfold tUnion. rewrite Union_commutative. 
    rewrite union_empty. constructor. }
-  {cleanup. instantiateHeap. instantiateContext. assert(tid:tid); repeat constructor. inversion H2; subst.
-   exists(tSingleton(tid,nil,nil,fill (handleCtxt x x0) (raise e))). 
-   exists(tSingleton(tid,nil,nil,fill x (app x0 e))). instantiatePool. repeat(split; try assumption). 
-   eraseEq. constructor. eraseEq. apply termErasePoolErase. eapply eraseFill; eauto. 
-   eapply pdecomposeDecomposed; eauto. rewrite <- ERASEHYP. constructor. econstructor. 
+  {cleanup. instantiateHeap. instantiateContext. inversion H0; subst. 
+   exists(tSingleton(Tid(0,0)nil,nil,nil,fill (handleCtxt x1 x0) (raise e))). 
+   exists(tSingleton(Tid(0,0)nil,nil,nil,fill x1 (app x0 e))). instantiatePool. repeat(split; try assumption). 
+   eraseEq. apply termErasePoolErase. apply pdecomposeEq in H4; subst. apply eraseFill; eauto. 
+   rewrite <- ERASEHYP. constructor. eraseEq. constructor. econstructor. 
    rewrite <- union_empty at 1. rewrite Union_commutative. reflexivity. proveDisjoint. eapply Handle. 
-   eapply decomposeDecomposed; eauto. unfold tUnion. rewrite Union_commutative. rewrite union_empty. 
+   eapply uneraseDecompose; eauto. unfold tUnion. rewrite Union_commutative. rewrite union_empty. 
    constructor. }
-  {cleanup. instantiateHeap. instantiateContext. assert(tid:tid); repeat constructor. inversion H2; subst.
-   exists(tSingleton(tid,nil,nil,fill (handleCtxt x x0) (ret e))). 
-   exists(tSingleton(tid,nil,nil,fill x (ret e))). instantiatePool. repeat(split; try assumption). 
-   eraseEq. constructor. eraseEq. apply termErasePoolErase. eapply eraseFill; eauto. 
-   apply pdecomposeDecomposed. auto. rewrite <- ERASEHYP. constructor. econstructor. 
+  {cleanup. instantiateHeap. instantiateContext. inversion H0; subst. 
+   exists(tSingleton(Tid(0,0)nil,nil,nil,fill (handleCtxt x1 x0) (ret e))). 
+   exists(tSingleton(Tid(0,0)nil,nil,nil,fill x1 (ret e))). instantiatePool. repeat(split; try assumption). 
+   eraseEq. apply termErasePoolErase. apply pdecomposeEq in H4; subst. apply eraseFill; eauto. 
+   rewrite <- ERASEHYP. constructor. eraseEq. constructor. econstructor. 
    rewrite <- union_empty at 1. rewrite Union_commutative. reflexivity. proveDisjoint. eapply HandleRet. 
-   eapply decomposeDecomposed; eauto. unfold tUnion. rewrite Union_commutative. rewrite union_empty. 
+   eapply uneraseDecompose; eauto. unfold tUnion. rewrite Union_commutative. rewrite union_empty. 
    constructor. }
-  {cleanup. instantiateHeap. instantiateContext. assert(tid:tid). repeat constructor.  
-   inversion H1; subst. exists (tSingleton(tid,nil,nil, fill x (fork e))). destruct tid. destruct p. 
-   exists (tCouple (Tid(n,S n0)l,nil,[fAct (Tid(1,1) ((n,n0)::l)) n0 (fill x (fork e))], 
-                    fill x (ret unit))(Tid(1,1)((n,n0)::l), nil,[specAct], e)). 
-   instantiatePool. repeat(split; try assumption). eraseEq. constructor. eraseEq.
-   apply termErasePoolCouple. eapply eraseFill. apply pdecomposeDecomposed. auto. auto. auto. auto. 
-   rewrite <- ERASEHYP. constructor. econstructor. rewrite <- union_empty at 1. rewrite Union_commutative. 
-   reflexivity. proveDisjoint. apply Fork. apply decomposeDecomposed; auto. reflexivity. 
-   econstructor. unfold tUnion. rewrite Union_commutative. rewrite union_empty.
+  {cleanup. instantiateHeap. instantiateContext. inversion H0; subst.
+   exists (tSingleton(Tid(0,0)nil,nil,nil, fill x0 (fork e))). 
+   exists (tCouple (Tid(0, 1)nil,nil,[fAct (Tid(1,1) [(0,0)]) 0 (fill x0 (fork e))], 
+                    fill x0 (ret unit)) (Tid(1,1)[(0,0)], nil,[specAct], e)). 
+   instantiatePool. repeat(split; try assumption). eraseEq. 
+   apply termErasePoolErase. apply pdecomposeEq in H4; subst. apply eraseFill; eauto. 
+   rewrite <- ERASEHYP. constructor. eraseEq. apply termErasePoolCouple; eauto. 
+   eapply eraseFill; eauto. rewrite <- ERASEHYP. constructor. econstructor. 
    rewrite <- union_empty at 1. rewrite Union_commutative. reflexivity. proveDisjoint. 
-   eapply PopFork. instantiate(4:=nil). reflexivity. instantiate(1:=nil). reflexivity. 
+   apply Fork. eapply uneraseDecompose; eauto. auto. econstructor. unfold tUnion. 
+   rewrite Union_commutative. rewrite union_empty.
+   rewrite <- union_empty at 1. rewrite Union_commutative. reflexivity. proveDisjoint. 
+   eapply PopFork. rewrite app_nil_l. reflexivity. rewrite app_nil_l. reflexivity. 
    unfold tUnion. rewrite Union_commutative. rewrite union_empty. constructor. }
   {cleanup. assert(exists H, speculateHeap PH' H). apply eHeap'.  invertExists. 
-   exists x0. copy H3. eapply lookupSpeculatedHeapFull with(x:=x) in H5; eauto. invertHyp. 
+   exists x0. eapply lookupSpeculatedHeapFull with(x:=x) in H5; eauto. invertHyp. 
    exists(replace x (sfull nil [Tid(0,0)nil] nil (Tid(0,0)nil) x1) x0). instantiateContext. 
-   exists (tSingleton(Tid(0,0)nil,nil,nil,fill x2 (get (fvar x)))). 
-   exists (tSingleton(bump (Tid(0,0)nil),nil, [rAct x 0 (fill x2 (get(fvar x)))], fill x2 (ret x1))). 
+   inversion H0; subst. inversion H7; subst. 
+   exists (tSingleton(Tid(0,0)nil,nil,nil,fill x3 (get (fvar x)))). 
+   exists (tSingleton(bump (Tid(0,0)nil),nil, [rAct x 0 (fill x3 (get(fvar x)))], fill x3 (ret x1))). 
    instantiatePool. repeat(split; try assumption). apply eraseSpeculatedHeap. assumption. 
    apply eraseHeapDependentReader; auto. apply eraseSpeculatedHeap. assumption. 
-   eraseEq. constructor. eraseEq. apply termErasePoolErase. eapply eraseFill; eauto.
-   apply pdecomposeDecomposed. auto. rewrite <- ERASEHYP. constructor. econstructor. 
+   eraseEq. apply termErasePoolErase. apply pdecomposeEq in H6; subst. apply eraseFill; eauto. 
+   rewrite <- ERASEHYP. constructor. eraseEq. constructor. econstructor. 
    rewrite <- union_empty at 1. rewrite Union_commutative. reflexivity. proveDisjoint. eapply Get. 
-   eapply decomposeDecomposed. eauto. eassumption. reflexivity. reflexivity. econstructor. reflexivity. 
-   proveDisjoint. eapply PopRead. instantiate (4:=nil). reflexivity. eapply HeapLookupReplace. eassumption. 
+   eapply uneraseDecompose; eauto. eauto. eauto. eauto. econstructor. reflexivity. 
+   proveDisjoint. eapply PopRead. rewrite app_nil_l. auto. eapply HeapLookupReplace. eassumption. 
    unfold tUnion. rewrite Union_commutative. rewrite union_empty. constructor. }
-  {cleanup. copy H1. assert(exists H, speculateHeap PH H). apply eHeap'. invertExists.  
-   exists x0. instantiateContext. assert(tid:tid). repeat constructor. 
-   inversion H4; subst. exists (replace x (sfull nil nil nil tid e) x0). destruct tid. destruct p.
-   inversion H11; subst. exists (tSingleton(Tid(n,n0)l,nil,nil,fill x1 (put (fvar x) e))). 
-   exists (tSingleton(Tid(n,S n0) l,nil,[wAct x n0 (fill x1 (put (fvar x) e))], fill x1 (ret unit))). 
+  {cleanup. assert(exists H, speculateHeap PH H). apply eHeap'. invertExists.  
+   exists x0. instantiateContext. inversion H0; subst. inversion H7; subst. 
+   exists (replace x (sfull nil nil nil (Tid(0,0)nil) e2) x0).
+   exists (tSingleton(Tid(0,0)nil,nil,nil,fill x2 (put (fvar x) e2))). 
+   exists (tSingleton(Tid(0,1)nil,nil,[wAct x 0 (fill x2 (put (fvar x) e2))], fill x2 (ret unit))). 
    instantiatePool. repeat (split; try assumption). apply eraseSpeculatedHeap. assumption. 
-   apply eraseReplaceSpecHeap; auto. eraseEq. constructor. eraseEq. 
-   apply termErasePoolErase. eapply eraseFill. apply pdecomposeDecomposed; auto. 
-   assumption. auto. rewrite <- ERASEHYP. constructor. econstructor. rewrite <- union_empty at 1. 
-   rewrite Union_commutative. reflexivity. proveDisjoint. eapply Put. eapply decomposeDecomposed. 
-   auto. eapply lookupSpeculatedHeapEmpty; eauto. reflexivity. reflexivity. econstructor. 
-   reflexivity. proveDisjoint. eapply PopWrite. instantiate(4:=nil). reflexivity. eapply HeapLookupReplace. 
-   eapply lookupSpeculatedHeapEmpty; eauto. reflexivity. unfold tUnion. rewrite Union_commutative. 
-   rewrite union_empty. constructor. }
+   apply eraseReplaceSpecHeap; auto. eraseEq. apply termErasePoolErase. apply pdecomposeEq in H2; subst. 
+   apply eraseFill; eauto. rewrite <- ERASEHYP. constructor. eraseEq. constructor. 
+   econstructor. rewrite <- union_empty at 1. rewrite Union_commutative. reflexivity. proveDisjoint. 
+   eapply Put. eapply uneraseDecompose; eauto. eapply lookupSpeculatedHeapEmpty; eauto. reflexivity. 
+   reflexivity. econstructor. reflexivity. proveDisjoint. eapply PopWrite. rewrite app_nil_l. auto. 
+   eapply HeapLookupReplace. eapply lookupSpeculatedHeapEmpty; eauto. reflexivity. unfold tUnion. 
+   rewrite Union_commutative. rewrite union_empty. constructor. }
   {cleanup. assert(exists H, speculateHeap PH H). apply eHeap'. invertExists. exists x0.
    assert(exists i newHeap', (i,newHeap') = extend (sempty nil) x0). 
    destruct x0; simpl; eauto. destruct p. eauto. invertHyp. exists x2. 
-   instantiateContext. exists(tSingleton(Tid(0,0)nil,nil,nil,fill x3 new)). 
-   exists (tSingleton(bump (Tid(0,0)nil),nil,[cAct x1 0 (fill x3 new)],fill x3 (ret (fvar x1)))). 
+   instantiateContext. exists(tSingleton(Tid(0,0)nil,nil,nil,fill x4 new)). 
+   exists (tSingleton(Tid(0,1)nil,nil,[cAct x1 0 (fill x4 new)],fill x4 (ret (fvar x)))). 
    instantiatePool. repeat(split; try assumption). eapply eraseSpeculatedHeap. assumption.
-   eapply eraseExtended; eauto.  
-   eraseEq. constructor. eraseEq. apply termErasePoolErase. eapply eraseFill. apply pdecomposeDecomposed. 
-   auto. assumption. constructor. assert(x=x1). eapply eraseExtended; eauto. subst. constructor. 
-   rewrite <- ERASEHYP. constructor. econstructor. 
-   rewrite <- union_empty at 1. rewrite Union_commutative. reflexivity. proveDisjoint. eapply New. 
-   apply decomposeDecomposed. auto. eassumption. reflexivity. econstructor. reflexivity. proveDisjoint. 
-   eapply PopNewEmpty. instantiate(4:=nil). reflexivity. eapply lookupExtend. eassumption. reflexivity. 
-   unfold tUnion. rewrite Union_commutative. rewrite union_empty. constructor. }
-  {cleanup. instantiateHeap. assert(exists M', eraseTerm M' tEmptySet M). apply eTerm. 
-   invertHyp. assert(tid:tid). repeat constructor. exists(tSingleton(tid,nil,nil,ret x)). 
+   eapply eraseExtended; eauto. eraseEq. apply termErasePoolErase. apply pdecomposeEq in H5; subst. 
+   apply eraseFill; eauto. rewrite <- ERASEHYP. constructor. eraseEq. constructor. 
+   econstructor. rewrite <- union_empty at 1. rewrite Union_commutative. reflexivity. proveDisjoint. eapply New.
+   eapply uneraseDecompose; eauto. eauto. eauto. econstructor. reflexivity. proveDisjoint. 
+   eapply PopNewEmpty. rewrite app_nil_l. auto. eapply lookupExtend. eassumption. reflexivity. 
+   unfold tUnion. rewrite Union_commutative. rewrite union_empty. 
+   eapply extendSpeculatedHeap in H1; eauto. subst. constructor. }
+  {cleanup. instantiateHeap. assert(exists M', uneraseTerm M M'). apply eUneraseTerm. 
+   invertHyp. exists(tSingleton(Tid(0,0)nil,nil,nil,ret x)). 
    exists tEmptySet. instantiatePool. repeat(split; try assumption). eraseEq. apply termErasePoolErase. 
-   constructor. assumption. rewrite <- ERASEHYP. constructor. eraseEq. apply Extensionality_Ensembles. 
+   auto. rewrite <- ERASEHYP. constructor. eraseEq. apply Extensionality_Ensembles. 
    unfold Same_set. unfold Included. split; intros. inversion H2. inversion H3. inversion H7. 
    inversion H2. rewrite <- ERASEHYP. constructor. econstructor. rewrite <- union_empty at 1. 
    rewrite Union_commutative. reflexivity. proveDisjoint. eapply Terminate. unfold tUnion. 
    rewrite union_empty. constructor. }
 Qed. 
    
+
+
+
+
+
+
+
+
+
+
